src/Refinements/BlockDiskRefinesItself.dfy
@@ -9,6 +9,8 @@ import A = BlockDisk
 import opened Block
 
 function IC(c: C.Constants): A.Constants
+    requires C.ConstantsValid(c)
+    ensures A.ConstantsValid(IC(c))
 {
     c
 }
@@ -27,14 +29,14 @@ lemma RefinesInit(c: C.Constants)
     ensures A.Valid(IC(c), I(c, C.Init(c)))
 {}
 
-lemma RefinesReadStep(c: C.Constants, s: C.State, s': C.State, block_id: int, val: Block.State)
+lemma RefinesReadStep(c: C.Constants, s: C.State, s': C.State, block_id: uint64, val: Block.State)
     requires C.NextStep(c, s, s', C.ReadBlock(block_id, val))
     requires C.Read(c, s, block_id) == val
     ensures A.Read(IC(c), I(c, s), block_id) == val
 {
 }
 
-lemma RefinesWriteStep(c: C.Constants, s: C.State, s': C.State, block_id: int, val: Block.State)
+lemma RefinesWriteStep(c: C.Constants, s: C.State, s': C.State, block_id: uint64, val: Block.State)
     requires C.NextStep(c, s, s', C.WriteBlock(block_id, val))
     requires C.Write(c, s, s', block_id, val)
     ensures A.Write(IC(c), I(c, s), I(c, s'), block_id, val)
